CoreLang/theories/Syntax.v
@@ -57,6 +57,18 @@ Inductive prim_op : Type :=
 
 #[global] Instance prim_op_eqdec : EqDecision prim_op. Proof. solve_decision. Defined.
 
+Inductive bin_op : Type :=
+  | bop_lt
+  | bop_le
+  | bop_gt
+  | bop_ge
+  | bop_plus
+  | bop_minus
+  | bop_and
+  | bop_or.
+
+#[global] Instance bin_op_eqdec : EqDecision bin_op. Proof. solve_decision. Defined.
+
 Definition base_ty_of_const (c : constant) : base_ty :=
   match c with
   | cbool _ => TBool
@@ -95,6 +107,7 @@ with tm : Type :=
   | tret    (v : value)
   | tlete   (e1 e2 : tm)
   | tprim   (op : prim_op) (arg : value)
+  | tbinop  (op : bin_op) (arg1 arg2 : value)
   | tapp    (v1 v2 : value)
   | tmatch  (v : value) (etrue efalse : tm)
   | tnode   (root left right : value)
@@ -113,7 +126,8 @@ with tm_eqdec' (e1 e2 : tm) : sumbool (e1 = e2) (e1 <> e2).
 Proof.
   - decide equality; try apply constant_eqdec; try apply ty_eqdec;
       try apply Nat.eq_dec; try solve_decision.
-  - decide equality; try apply prim_op_eqdec; try solve_decision.
+  - decide equality; try apply prim_op_eqdec; try apply bin_op_eqdec;
+      try solve_decision.
 Defined.
 
 #[global] Instance value_eqdec : EqDecision value := value_eqdec'.
@@ -137,6 +151,7 @@ with open_tm (k : nat) (s : value) (e : tm) : tm :=
   | tret v          => tret (open_value k s v)
   | tlete e1 e2     => tlete (open_tm k s e1) (open_tm (S k) s e2)
   | tprim op v      => tprim op (open_value k s v)
+  | tbinop op v1 v2 => tbinop op (open_value k s v1) (open_value k s v2)
   | tapp v1 v2      => tapp (open_value k s v1) (open_value k s v2)
   | tmatch v et ef  =>
       tmatch (open_value k s v) (open_tm k s et) (open_tm k s ef)
@@ -193,6 +208,7 @@ with close_tm (x : atom) (k : nat) (e : tm) : tm :=
   | tret v          => tret (close_value x k v)
   | tlete e1 e2     => tlete (close_tm x k e1) (close_tm x (S k) e2)
   | tprim op v      => tprim op (close_value x k v)
+  | tbinop op v1 v2 => tbinop op (close_value x k v1) (close_value x k v2)
   | tapp v1 v2      => tapp (close_value x k v1) (close_value x k v2)
   | tmatch v et ef  =>
       tmatch (close_value x k v) (close_tm x k et) (close_tm x k ef)
@@ -226,6 +242,7 @@ with fv_tm (e : tm) : aset :=
   | tret v          => fv_value v
   | tlete e1 e2     => fv_tm e1 ∪ fv_tm e2
   | tprim _ v       => fv_value v
+  | tbinop _ v1 v2  => fv_value v1 ∪ fv_value v2
   | tapp v1 v2      => fv_value v1 ∪ fv_value v2
   | tmatch v et ef  => fv_value v ∪ fv_tm et ∪ fv_tm ef
   | tnode r l rr => fv_value r ∪ fv_value l ∪ fv_value rr
@@ -264,6 +281,7 @@ with tm_lvars_at (d : nat) (e : tm) : lvset :=
   | tret v => value_lvars_at d v
   | tlete e1 e2 => tm_lvars_at d e1 ∪ tm_lvars_at (S d) e2
   | tprim _ v => value_lvars_at d v
+  | tbinop _ v1 v2 => value_lvars_at d v1 ∪ value_lvars_at d v2
   | tapp v1 v2 => value_lvars_at d v1 ∪ value_lvars_at d v2
   | tmatch v et ef =>
       value_lvars_at d v ∪ tm_lvars_at d et ∪ tm_lvars_at d ef
@@ -302,6 +320,8 @@ with tm_swap_atom (x y : atom) (e : tm) : tm :=
   | tret v => tret (value_swap_atom x y v)
   | tlete e1 e2 => tlete (tm_swap_atom x y e1) (tm_swap_atom x y e2)
   | tprim op v => tprim op (value_swap_atom x y v)
+  | tbinop op v1 v2 =>
+      tbinop op (value_swap_atom x y v1) (value_swap_atom x y v2)
   | tapp v1 v2 => tapp (value_swap_atom x y v1) (value_swap_atom x y v2)
   | tmatch v et ef =>
       tmatch (value_swap_atom x y v)
@@ -332,6 +352,7 @@ Proof.
     + apply fv_value_swap_atom.
     + rewrite !fv_tm_swap_atom. better_base_solver.
     + apply fv_value_swap_atom.
+    + rewrite !fv_value_swap_atom. better_base_solver.
     + rewrite !fv_value_swap_atom. better_base_solver.
     + rewrite fv_value_swap_atom, !fv_tm_swap_atom. better_base_solver.
     + rewrite !fv_value_swap_atom. better_base_solver.
@@ -436,6 +457,7 @@ with tm_subst (x : atom) (s : value) (e : tm) : tm :=
   | tret v          => tret (value_subst x s v)
   | tlete e1 e2     => tlete (tm_subst x s e1) (tm_subst x s e2)
   | tprim op v      => tprim op (value_subst x s v)
+  | tbinop op v1 v2 => tbinop op (value_subst x s v1) (value_subst x s v2)
   | tapp v1 v2      => tapp (value_subst x s v1) (value_subst x s v2)
   | tmatch v et ef  =>
       tmatch (value_subst x s v) (tm_subst x s et) (tm_subst x s ef)
@@ -494,6 +516,9 @@ with lc_tm : tm → Prop :=
   | LC_op op v :
       lc_value v →
       lc_tm (tprim op v)
+  | LC_binop op v1 v2 :
+      lc_value v1 → lc_value v2 →
+      lc_tm (tbinop op v1 v2)
   | LC_app v1 v2 :
       lc_value v1 → lc_value v2 →
       lc_tm (tapp v1 v2)
