CaseStudy/theories/Section2Typing.v
@@ -1,0 +1,218 @@
+(** * Small programs from Section 2 (typing overview) *)
+
+From ProofAutomation Require Import BasicTypeInfer ExtendedTypeInfer.
+
+Open Scope case_scope.
+Open Scope core_scope.
+Open Scope cty_scope.
+
+Section Section2TypingExamples.
+
+Definition x : atom := 201%positive.
+Definition y : atom := 202%positive.
+Definition z : atom := 203%positive.
+Definition g : atom := 204%positive.
+Definition gx : atom := 205%positive.
+Definition cmp : atom := 206%positive.
+Definition ylet : atom := 207%positive.
+Definition cond : atom := 208%positive.
+Definition c1 : atom := 209%positive.
+Definition c2 : atom := 210%positive.
+Definition f : atom := 211%positive.
+Definition a : atom := 212%positive.
+Definition r1 : atom := 213%positive.
+Definition r2 : atom := 214%positive.
+
+Definition one_program : tm :=
+  ret (vnat 1).
+
+Definition minus_three_program : tm :=
+  ret (ƛ x : ℕ => x ⟨ - ⟩ vnat 3).
+
+Definition x_minus_three : tm :=
+  x ⟨ - ⟩ vnat 3.
+
+Definition may_must_intro_program : tm :=
+  ret (ƛ g : ℕ →ᵦ ℕ =>
+    ret (ƛ x : ℕ =>
+      ret (ƛ y : ℕ =>
+        let cond := y ⟨ > ⟩ vnat 10 in
+        if cond then
+          let gx := g @ x in
+          gx ⟨ + ⟩ vnat 1
+        else
+          x ⟨ + ⟩ vnat 1))).
+
+Definition dependent_context_program : tm :=
+  let x := op_natGen ·₁ vnat 0 in
+  let y := x ⟨ + ⟩ vnat 1 in
+  x ⟨ - ⟩ y.
+
+Definition independent_context_program : tm :=
+  let x := op_natGen ·₁ vnat 0 in
+  let y := op_natGen ·₁ vnat 0 in
+  x ⟨ - ⟩ y.
+
+Definition x_minus_y : tm :=
+  x ⟨ - ⟩ y.
+
+Definition x_minus_z_plus_y : tm :=
+  let a := z ⟨ + ⟩ y in
+  x ⟨ - ⟩ a.
+
+Definition y_minus_z : tm :=
+  y ⟨ - ⟩ z.
+
+Definition branch_three_five : tm :=
+  let cond := op_eq0 ·₁ x in
+  if cond then ret (vnat 3) else ret (vnat 5).
+
+Definition branch_five_three : tm :=
+  let cond := x ⟨ > ⟩ vnat 0 in
+  if cond then ret (vnat 5) else ret (vnat 3).
+
+Definition let_duplication_program : tm :=
+  let ylet := x ⟨ - ⟩ vnat 3 in
+  x ⟨ - ⟩ ylet.
+
+Definition minus_curried_program : tm :=
+  ret (ƛ x : ℕ =>
+    ret (ƛ y : ℕ => x ⟨ - ⟩ y)).
+
+Definition nested_apply_program : tm :=
+  ret (ƛ f : ℕ →ᵦ ℕ =>
+    let r1 := f @ y in
+    let r2 := f @ r1 in
+    x ⟨ - ⟩ r2).
+
+Definition ack_like_program : tm :=
+  ret (μ f, x : ℕ ~> ℕ →ᵦ ℕ =>
+    ret (ƛ y : ℕ =>
+      let c1 := op_eq0 ·₁ x in
+      if c1 then
+        ret (vnat 0)
+      else
+        let c2 := op_eq0 ·₁ y in
+        if c2 then
+          ret x
+        else
+          let r1 := x ⟨ - ⟩ vnat 1 in
+          let r2 := y ⟨ - ⟩ vnat 1 in
+          f @@ (r1, r2))).
+
+Definition nat_match_like_program : tm :=
+  let cond := op_eq0 ·₁ x in
+  if cond then ret (vnat 3) else ret (vnat 5).
+
+Definition nat_to_nat_ty : ty := (ℕ : ty) →ᵦ ℕ.
+Definition nat_to_nat_to_nat_ty : ty := (ℕ : ty) →ᵦ ℕ →ᵦ ℕ.
+Definition may_must_intro_basic_ty : ty :=
+  (ℕ →ᵦ ℕ) →ᵦ ℕ →ᵦ ℕ →ᵦ ℕ.
+
+Lemma one_program_basic_type :
+  ∅ ⊢ₑ one_program ⋮ ℕ.
+Proof. unfold one_program. basic_check. Qed.
+
+Lemma one_program_extended_type :
+  ∅; Emp ⊢ₓ one_program ⋮ const_precise_ty (cnat 1).
+Proof.
+  unfold one_program.
+  eapply EXT_Const.
+  extended_wf.
+Qed.
+
+Lemma minus_three_program_basic_type :
+  ∅ ⊢ₑ minus_three_program ⋮ nat_to_nat_ty.
+Proof. unfold minus_three_program, nat_to_nat_ty. basic_check. Qed.
+
+Lemma x_minus_three_basic_type :
+  <[x := (ℕ : ty)]> ∅ ⊢ₑ x_minus_three ⋮ ℕ.
+Proof. unfold x_minus_three. basic_check. Qed.
+
+Lemma x_minus_three_extended_type :
+  ∅; x ∷ ONat ⊢ₓ
+    x_minus_three ⋮ binop_precise_ty bop_minus (avar x) (vnat 3).
+Proof.
+  unfold x_minus_three.
+  eapply EXT_BinOp.
+  extended_wf.
+Qed.
+
+Lemma may_must_intro_program_basic_type :
+  ∅ ⊢ₑ may_must_intro_program ⋮ may_must_intro_basic_ty.
+Proof. unfold may_must_intro_program, may_must_intro_basic_ty. basic_check. Qed.
+
+Lemma dependent_context_program_basic_type :
+  ∅ ⊢ₑ dependent_context_program ⋮ ℕ.
+Proof. unfold dependent_context_program. basic_check. Qed.
+
+Lemma independent_context_program_basic_type :
+  ∅ ⊢ₑ independent_context_program ⋮ ℕ.
+Proof. unfold independent_context_program. basic_check. Qed.
+
+Lemma x_minus_y_basic_type :
+  <[y := (ℕ : ty)]> (<[x := (ℕ : ty)]> ∅) ⊢ₑ x_minus_y ⋮ ℕ.
+Proof. unfold x_minus_y. basic_check. Qed.
+
+Lemma x_minus_y_extended_type :
+  ∅; (x ∷ ONat) ,, (y ∷ ONat) ⊢ₓ
+    x_minus_y ⋮ binop_precise_ty bop_minus (avar x) (avar y).
+Proof.
+  unfold x_minus_y.
+  eapply EXT_BinOp.
+  extended_wf.
+Qed.
+
+Lemma x_minus_z_plus_y_basic_type :
+  <[z := (ℕ : ty)]> (<[y := (ℕ : ty)]> (<[x := (ℕ : ty)]> ∅)) ⊢ₑ x_minus_z_plus_y ⋮ ℕ.
+Proof. unfold x_minus_z_plus_y. basic_check. Qed.
+
+Lemma y_minus_z_basic_type :
+  <[z := (ℕ : ty)]> (<[y := (ℕ : ty)]> ∅) ⊢ₑ y_minus_z ⋮ ℕ.
+Proof. unfold y_minus_z. basic_check. Qed.
+
+Lemma y_minus_z_extended_type :
+  ∅; (y ∷ ONat) ,, (z ∷ ONat) ⊢ₓ
+    y_minus_z ⋮ binop_precise_ty bop_minus (avar y) (avar z).
+Proof.
+  unfold y_minus_z.
+  eapply EXT_BinOp.
+  extended_wf.
+Qed.
+
+Lemma branch_three_five_basic_type :
+  <[x := (ℕ : ty)]> ∅ ⊢ₑ branch_three_five ⋮ ℕ.
+Proof. unfold branch_three_five. basic_check. Qed.
+
+Lemma branch_five_three_basic_type :
+  <[x := (ℕ : ty)]> ∅ ⊢ₑ branch_five_three ⋮ ℕ.
+Proof. unfold branch_five_three. basic_check. Qed.
+
+Lemma let_duplication_program_basic_type :
+  <[x := (ℕ : ty)]> ∅ ⊢ₑ let_duplication_program ⋮ ℕ.
+Proof. unfold let_duplication_program. basic_check. Qed.
+
+Lemma minus_curried_program_basic_type :
+  ∅ ⊢ₑ minus_curried_program ⋮ nat_to_nat_to_nat_ty.
+Proof. unfold minus_curried_program, nat_to_nat_to_nat_ty. basic_check. Qed.
+
+Lemma nested_apply_program_basic_type :
+  <[y := (ℕ : ty)]> (<[x := (ℕ : ty)]> ∅) ⊢ₑ
+    nested_apply_program ⋮ ((ℕ →ᵦ ℕ) →ᵦ ℕ).
+Proof.
+  unfold nested_apply_program, nat_to_nat_ty.
+  basic_check.
+Qed.
+
+Lemma ack_like_program_basic_type :
+  ∅ ⊢ₑ ack_like_program ⋮ nat_to_nat_to_nat_ty.
+Proof.
+  unfold ack_like_program, nat_to_nat_to_nat_ty.
+  basic_check.
+Qed.
+
+Lemma nat_match_like_program_basic_type :
+  <[x := (ℕ : ty)]> ∅ ⊢ₑ nat_match_like_program ⋮ ℕ.
+Proof. unfold nat_match_like_program. basic_check. Qed.
+
+End Section2TypingExamples.
