CaseStudy/theories/Section3Logic.v
@@ -1,0 +1,76 @@
+(** * Small program witnesses for Section 3 (logic and denotation) *)
+
+From ProofAutomation Require Import BasicTypeInfer ExtendedTypeInfer.
+
+Open Scope case_scope.
+Open Scope core_scope.
+Open Scope cty_scope.
+
+Section Section3LogicExamples.
+
+Definition x : atom := 301%positive.
+Definition y : atom := 302%positive.
+Definition p : atom := 303%positive.
+Definition q : atom := 304%positive.
+Definition c : atom := 305%positive.
+
+Definition logic_project_x : tm :=
+  ret x.
+
+Definition logic_correlated_xy : tm :=
+  let y := x ⟨ + ⟩ vnat 1 in
+  x ⟨ + ⟩ y.
+
+Definition logic_branch_atom_example : tm :=
+  let c := x ⟨ ≤ ⟩ vnat 2 in
+  if c then
+    ret x
+  else
+    y ⟨ + ⟩ vnat 1.
+
+Definition logic_product_style_example : tm :=
+  x ⟨ + ⟩ y.
+
+Definition logic_implication_witness : tm :=
+  ret (ƛ x : ℕ => x ⟨ + ⟩ vnat 1).
+
+Definition nat_increment_ty : ty := (ℕ : ty) →ᵦ ℕ.
+
+Lemma logic_project_x_basic_type :
+  <[x := (ℕ : ty)]> ∅ ⊢ₑ logic_project_x ⋮ ℕ.
+Proof. unfold logic_project_x. basic_check. Qed.
+
+Lemma logic_project_x_extended_type :
+  ∅; x ∷ ONat ⊢ₓ logic_project_x ⋮ ONat.
+Proof.
+  unfold logic_project_x.
+  eapply EXT_Var.
+  extended_wf.
+Qed.
+
+Lemma logic_correlated_xy_basic_type :
+  <[x := (ℕ : ty)]> ∅ ⊢ₑ logic_correlated_xy ⋮ ℕ.
+Proof. unfold logic_correlated_xy. basic_check. Qed.
+
+Lemma logic_branch_atom_example_basic_type :
+  <[y := (ℕ : ty)]> (<[x := (ℕ : ty)]> ∅) ⊢ₑ logic_branch_atom_example ⋮ ℕ.
+Proof. unfold logic_branch_atom_example. basic_check. Qed.
+
+Lemma logic_product_style_example_basic_type :
+  <[y := (ℕ : ty)]> (<[x := (ℕ : ty)]> ∅) ⊢ₑ logic_product_style_example ⋮ ℕ.
+Proof. unfold logic_product_style_example. basic_check. Qed.
+
+Lemma logic_product_style_example_extended_type :
+  ∅; (x ∷ ONat) ,, (y ∷ ONat) ⊢ₓ
+    logic_product_style_example ⋮ binop_precise_ty bop_plus (avar x) (avar y).
+Proof.
+  unfold logic_product_style_example.
+  eapply EXT_BinOp.
+  extended_wf.
+Qed.
+
+Lemma logic_implication_witness_basic_type :
+  ∅ ⊢ₑ logic_implication_witness ⋮ nat_increment_ty.
+Proof. unfold logic_implication_witness, nat_increment_ty. basic_check. Qed.
+
+End Section3LogicExamples.
