CaseStudy/theories/Section4Extension.v
@@ -1,0 +1,162 @@
+(** * Small programs from Section 4 (nondeterminism and persistence) *)
+
+From ProofAutomation Require Import BasicTypeInfer ExtendedTypeInfer.
+
+Open Scope case_scope.
+Open Scope core_scope.
+Open Scope cty_scope.
+
+Section Section4ExtensionExamples.
+
+Definition z : atom := 401%positive.
+Definition x : atom := 402%positive.
+Definition y : atom := 403%positive.
+Definition f : atom := 404%positive.
+Definition y1 : atom := 405%positive.
+Definition y2 : atom := 406%positive.
+Definition r : atom := 407%positive.
+Definition c : atom := 408%positive.
+Definition c1 : atom := 409%positive.
+Definition c2 : atom := 410%positive.
+
+Definition bool_gen_program : tm :=
+  op_boolGen ·₁ vbool false.
+
+Definition nat_gen_program : tm :=
+  op_natGen ·₁ vnat 0.
+
+Definition nondet_choice_program : tm :=
+  ret (vnat 0) ⊕ₙ ret (vnat 1).
+
+Definition envir_x_program : tm :=
+  let x := nat_gen_program in
+  x ⟨ + ⟩ vnat 1.
+
+Definition captured_z_fun : tm :=
+  ret (ƛ x : 𝔹 => ret z).
+
+Definition double_call_captured_z : tm :=
+  let f := captured_z_fun in
+  let y1 := f @ vbool true in
+  let y2 := f @ vbool false in
+  ret y2.
+
+Definition nat_gen_fun : tm :=
+  ret (ƛ x : 𝔹 => nat_gen_program).
+
+Definition choice_fun : tm :=
+  ret (ƛ x : 𝔹 => ret (vnat 0)) ⊕ₙ
+  ret (ƛ x : 𝔹 => nat_gen_program).
+
+Definition nonpersistent_choice_use : tm :=
+  let f := choice_fun in
+  let r := f @ vbool true in
+  let c := op_eq0 ·₁ r in
+  if c then
+    f @ vbool false
+  else
+    ret (vnat 0).
+
+Definition bool_equality_body : tm :=
+  if y then
+    if x then ret (vbool true) else ret (vbool false)
+  else
+    if x then ret (vbool false) else ret (vbool true).
+
+Definition bool_gen_closure_program : tm :=
+  let x := bool_gen_program in
+  ret (ƛ y : 𝔹 => bool_equality_body).
+
+Definition bool_gen_sum_program : tm :=
+  bool_gen_program.
+
+Definition bool_to_nat_ty : ty := (𝔹 : ty) →ᵦ ℕ.
+Definition bool_to_bool_ty : ty := (𝔹 : ty) →ᵦ 𝔹.
+
+Lemma bool_gen_program_basic_type :
+  ∅ ⊢ₑ bool_gen_program ⋮ 𝔹.
+Proof. unfold bool_gen_program. basic_check. Qed.
+
+Lemma bool_gen_program_extended_type :
+  ∅; Emp ⊢ₓ bool_gen_program ⋮
+    primop_precise_ty op_boolGen (vbool false).
+Proof. unfold bool_gen_program. eapply EXT_AppOpValue. extended_wf. Qed.
+
+Lemma nat_gen_program_basic_type :
+  ∅ ⊢ₑ nat_gen_program ⋮ ℕ.
+Proof. unfold nat_gen_program. basic_check. Qed.
+
+Lemma nat_gen_program_extended_type :
+  ∅; Emp ⊢ₓ nat_gen_program ⋮
+    primop_precise_ty op_natGen (vnat 0).
+Proof. unfold nat_gen_program. eapply EXT_AppOpValue. extended_wf. Qed.
+
+Lemma nondet_choice_program_basic_type :
+  ∅ ⊢ₑ nondet_choice_program ⋮ ℕ.
+Proof. unfold nondet_choice_program. basic_check. Qed.
+
+Lemma envir_x_program_basic_type :
+  ∅ ⊢ₑ envir_x_program ⋮ ℕ.
+Proof. unfold envir_x_program, nat_gen_program. basic_check. Qed.
+
+Lemma captured_z_fun_basic_type :
+  <[z := (ℕ : ty)]> ∅ ⊢ₑ captured_z_fun ⋮ bool_to_nat_ty.
+Proof. unfold captured_z_fun, bool_to_nat_ty. basic_check. Qed.
+
+Lemma double_call_captured_z_basic_type :
+  <[z := (ℕ : ty)]> ∅ ⊢ₑ double_call_captured_z ⋮ ℕ.
+Proof.
+  unfold double_call_captured_z, bool_to_nat_ty.
+  eapply basic_typing_let_named.
+  - basic_type_fresh.
+  - apply captured_z_fun_basic_type.
+  - eapply basic_typing_let_named.
+    + basic_type_fresh.
+    + basic_check.
+    + eapply basic_typing_let_named.
+      * basic_type_fresh.
+      * basic_check.
+      * basic_check.
+Qed.
+
+Lemma nat_gen_fun_basic_type :
+  ∅ ⊢ₑ nat_gen_fun ⋮ bool_to_nat_ty.
+Proof. unfold nat_gen_fun, nat_gen_program, bool_to_nat_ty. basic_check. Qed.
+
+Lemma choice_fun_basic_type :
+  ∅ ⊢ₑ choice_fun ⋮ bool_to_nat_ty.
+Proof. unfold choice_fun, nat_gen_program, bool_to_nat_ty. basic_check. Qed.
+
+Lemma nonpersistent_choice_use_basic_type :
+  ∅ ⊢ₑ nonpersistent_choice_use ⋮ ℕ.
+Proof.
+  unfold nonpersistent_choice_use.
+  eapply basic_typing_let_named.
+  - basic_type_fresh.
+  - apply choice_fun_basic_type.
+  - eapply basic_typing_let_named.
+    + basic_type_fresh.
+    + basic_check.
+    + eapply basic_typing_let_named.
+      * basic_type_fresh.
+      * basic_check.
+      * basic_check.
+Qed.
+
+Lemma bool_equality_body_basic_type :
+  <[y := (𝔹 : ty)]> (<[x := (𝔹 : ty)]> ∅) ⊢ₑ bool_equality_body ⋮ 𝔹.
+Proof. unfold bool_equality_body. basic_check. Qed.
+
+Lemma bool_gen_closure_program_basic_type :
+  ∅ ⊢ₑ bool_gen_closure_program ⋮ bool_to_bool_ty.
+Proof.
+  unfold bool_gen_closure_program, bool_gen_program, bool_equality_body,
+    bool_to_bool_ty.
+  basic_check.
+Qed.
+
+Lemma bool_gen_sum_program_basic_type :
+  ∅ ⊢ₑ bool_gen_sum_program ⋮ 𝔹.
+Proof. unfold bool_gen_sum_program, bool_gen_program. basic_check. Qed.
+
+End Section4ExtensionExamples.
