ContextBasicDenotation/theories/TermSyntax.v
@@ -43,6 +43,7 @@ Proof.
   - rewrite lvars_fv_union, H, H0. reflexivity.
   - apply H.
   - rewrite lvars_fv_union, H, H0. reflexivity.
+  - rewrite lvars_fv_union, H, H0. reflexivity.
 	  - rewrite !lvars_fv_union, H, H0, H1. set_solver.
 	  - rewrite !lvars_fv_union, H, H0, H1. set_solver.
 	  - rewrite !lvars_fv_union, H, H0, H1. set_solver.
@@ -111,6 +112,7 @@ Proof.
   - rewrite lvars_at_depth_union, H, H0.
     replace (S c + d) with (S (c + d)) by lia. reflexivity.
   - rewrite H. reflexivity.
+  - rewrite lvars_at_depth_union, H, H0. reflexivity.
   - rewrite lvars_at_depth_union, H, H0. reflexivity.
   - rewrite !lvars_at_depth_union, H, H0, H1. reflexivity.
   - rewrite !lvars_at_depth_union, H, H0, H1. reflexivity.
@@ -188,6 +190,9 @@ Proof.
     rewrite H0 by (rewrite ?lvars_fv_union in *; set_solver).
     rewrite <- set_swap_union. reflexivity.
   - apply H. exact H0.
+  - rewrite H by (rewrite ?lvars_fv_union in *; set_solver).
+    rewrite H0 by (rewrite ?lvars_fv_union in *; set_solver).
+    rewrite <- set_swap_union. reflexivity.
   - rewrite H by (rewrite ?lvars_fv_union in *; set_solver).
     rewrite H0 by (rewrite ?lvars_fv_union in *; set_solver).
     rewrite <- set_swap_union. reflexivity.
@@ -328,6 +333,7 @@ Proof.
     (fun v Hlc IH => IH)
     (fun e1 e2 L Hlc1 IH1 Hbody IH2 => _)
 	    (fun op v Hlc IH => IH)
+	    (fun op v1 v2 Hlc1 IH1 Hlc2 IH2 => _)
 	    (fun v1 v2 Hlc1 IH1 Hlc2 IH2 => _)
 	    (fun v et ef Hlcv IHv Hlcet IHet Hlcef IHef => _)
 	    (fun root left right Hlcroot IHroot Hlcleft IHleft Hlcright IHright => _)
@@ -379,10 +385,14 @@ Proof.
     assert (Hdepth : lvars_bv (lvars_at_depth 1 (tm_lvars e2)) = ∅).
     { apply lvars_bv_at_depth_succ_empty_of_open0 with (x := x). exact IH2. }
     rewrite Hdepth. set_solver.
-  - cbn [value_lvars tm_lvars value_lvars_at tm_lvars_at].
-    change (value_lvars_at 0 v1) with (value_lvars v1).
-    change (value_lvars_at 0 v2) with (value_lvars v2).
-    rewrite lvars_bv_union, IH1, IH2. set_solver.
+	  - cbn [value_lvars tm_lvars value_lvars_at tm_lvars_at].
+	    change (value_lvars_at 0 v1) with (value_lvars v1).
+	    change (value_lvars_at 0 v2) with (value_lvars v2).
+	    rewrite lvars_bv_union, IH1, IH2. set_solver.
+	  - cbn [value_lvars tm_lvars value_lvars_at tm_lvars_at].
+	    change (value_lvars_at 0 v1) with (value_lvars v1).
+	    change (value_lvars_at 0 v2) with (value_lvars v2).
+	    rewrite lvars_bv_union, IH1, IH2. set_solver.
   - cbn [value_lvars tm_lvars value_lvars_at tm_lvars_at].
     change (value_lvars_at 0 v) with (value_lvars v).
     change (tm_lvars_at 0 et) with (tm_lvars et).
@@ -725,12 +735,15 @@ Proof.
     + apply H. rewrite lvars_bv_union in H1. set_solver.
     + apply H0. rewrite lvars_bv_union in H1. set_solver.
   - f_equal. apply H. exact H0.
-  - f_equal.
-    + apply H. rewrite lvars_bv_union in H1. set_solver.
-    + apply H0. rewrite lvars_bv_union in H1. set_solver.
-  - f_equal.
-    + apply H. rewrite !lvars_bv_union in H2. set_solver.
-    + apply H0. rewrite !lvars_bv_union in H2. set_solver.
+	  - f_equal.
+	    + apply H. rewrite lvars_bv_union in H1. set_solver.
+	    + apply H0. rewrite lvars_bv_union in H1. set_solver.
+	  - f_equal.
+	    + apply H. rewrite lvars_bv_union in H1. set_solver.
+	    + apply H0. rewrite lvars_bv_union in H1. set_solver.
+	  - f_equal.
+	    + apply H. rewrite !lvars_bv_union in H2. set_solver.
+	    + apply H0. rewrite !lvars_bv_union in H2. set_solver.
     + apply H1. rewrite !lvars_bv_union in H2. set_solver.
   - f_equal.
     + apply H. rewrite !lvars_bv_union in H2. set_solver.
@@ -951,10 +964,12 @@ Proof.
   - rewrite H by exact H1.
     rewrite H0 by lia. reflexivity.
   - rewrite H by exact H0. reflexivity.
-  - rewrite H by exact H1.
-    rewrite H0 by exact H1. reflexivity.
-  - rewrite H by exact H2.
-    rewrite H0 by exact H2.
+	  - rewrite H by exact H1.
+	    rewrite H0 by exact H1. reflexivity.
+	  - rewrite H by exact H1.
+	    rewrite H0 by exact H1. reflexivity.
+	  - rewrite H by exact H2.
+	    rewrite H0 by exact H2.
     rewrite H1 by exact H2. reflexivity.
   - rewrite (H d k H2).
     rewrite (H0 d k H2).
@@ -1007,12 +1022,16 @@ Proof.
   - rewrite value_lvars_at_shift_under by lia.
     cbn [tm_lvars_at].
     rewrite !value_lvars_at_bound0_under. set_solver.
-  - rewrite value_lvars_at_shift_under by lia.
-    rewrite value_lvars_at_shift_under by lia.
-    cbn [tm_lvars_at].
-    rewrite !value_lvars_at_bound0_under. set_solver.
-  - rewrite value_lvars_at_shift_under by lia.
-    rewrite tm_lvars_at_shift_under by lia.
+	  - rewrite value_lvars_at_shift_under by lia.
+	    rewrite value_lvars_at_shift_under by lia.
+	    cbn [tm_lvars_at].
+	    rewrite !value_lvars_at_bound0_under. set_solver.
+	  - rewrite value_lvars_at_shift_under by lia.
+	    rewrite value_lvars_at_shift_under by lia.
+	    cbn [tm_lvars_at].
+	    rewrite !value_lvars_at_bound0_under. set_solver.
+	  - rewrite value_lvars_at_shift_under by lia.
+	    rewrite tm_lvars_at_shift_under by lia.
     rewrite tm_lvars_at_shift_under by lia.
     cbn [tm_lvars_at].
     rewrite !value_lvars_at_bound0_under. set_solver.
@@ -1072,10 +1091,13 @@ with lstore_instantiate_tm_split_at
   | tlete e1 e2 =>
       tlete (lstore_instantiate_tm_split_at d σf σb e1)
         (lstore_instantiate_tm_split_at (S d) σf σb e2)
-  | tprim op v => tprim op (lstore_instantiate_value_split_at d σf σb v)
-  | tapp v1 v2 =>
-      tapp (lstore_instantiate_value_split_at d σf σb v1)
-        (lstore_instantiate_value_split_at d σf σb v2)
+	  | tprim op v => tprim op (lstore_instantiate_value_split_at d σf σb v)
+	  | tbinop op v1 v2 =>
+	      tbinop op (lstore_instantiate_value_split_at d σf σb v1)
+	        (lstore_instantiate_value_split_at d σf σb v2)
+	  | tapp v1 v2 =>
+	      tapp (lstore_instantiate_value_split_at d σf σb v1)
+	        (lstore_instantiate_value_split_at d σf σb v2)
 	  | tmatch v et ef =>
 	      tmatch (lstore_instantiate_value_split_at d σf σb v)
 	        (lstore_instantiate_tm_split_at d σf σb et)
@@ -1199,9 +1221,10 @@ Proof.
   - f_equal. apply H. exact H0.
   - f_equal. apply H. exact H0.
   - f_equal; [apply H | apply H0]; set_solver.
-  - f_equal. apply H. exact H0.
-  - f_equal; [apply H | apply H0]; set_solver.
-  - f_equal; [apply H | apply H0 | apply H1]; set_solver.
+	  - f_equal. apply H. exact H0.
+	  - f_equal; [apply H | apply H0]; set_solver.
+	  - f_equal; [apply H | apply H0]; set_solver.
+	  - f_equal; [apply H | apply H0 | apply H1]; set_solver.
   - f_equal; [apply H | apply H0 | apply H1]; set_solver.
   - f_equal; [apply H | apply H0 | apply H1]; set_solver.
   - f_equal; [apply H | apply H0]; set_solver.
@@ -1280,9 +1303,10 @@ Proof.
   - f_equal. apply H. exact H0.
   - f_equal. apply H. exact H0.
   - f_equal; [apply H | apply H0]; set_solver.
-  - f_equal. apply H. exact H0.
-  - f_equal; [apply H | apply H0]; set_solver.
-  - f_equal; [apply H | apply H0 | apply H1]; set_solver.
+	  - f_equal. apply H. exact H0.
+	  - f_equal; [apply H | apply H0]; set_solver.
+	  - f_equal; [apply H | apply H0]; set_solver.
+	  - f_equal; [apply H | apply H0 | apply H1]; set_solver.
   - f_equal; [apply H | apply H0 | apply H1]; set_solver.
   - f_equal; [apply H | apply H0 | apply H1]; set_solver.
   - f_equal; [apply H | apply H0]; set_solver.
@@ -1336,10 +1360,11 @@ Proof.
 	    end.
   - rewrite subst_map_vlam. f_equal. apply H. exact H0.
   - rewrite subst_map_vfix. f_equal. apply H. exact H0.
-  - rewrite subst_map_ret. f_equal. apply H. exact H0.
-  - rewrite subst_map_lete. f_equal; [apply H | apply H0]; exact H1.
-  - rewrite subst_map_tprim. f_equal. apply H. exact H0.
-  - rewrite subst_map_tapp. f_equal; [apply H | apply H0]; exact H1.
+	  - rewrite subst_map_ret. f_equal. apply H. exact H0.
+	  - rewrite subst_map_lete. f_equal; [apply H | apply H0]; exact H1.
+	  - rewrite subst_map_tprim. f_equal. apply H. exact H0.
+	  - rewrite subst_map_tbinop. f_equal; [apply H | apply H0]; exact H1.
+	  - rewrite subst_map_tapp. f_equal; [apply H | apply H0]; exact H1.
   - rewrite subst_map_tmatch. repeat f_equal;
       [apply H | apply H0 | apply H1]; exact H2.
   - rewrite subst_map_tnode. repeat f_equal;
@@ -1416,9 +1441,10 @@ Proof.
   - f_equal. apply H; set_solver.
   - f_equal. apply H; set_solver.
   - f_equal; [apply H | apply H0]; set_solver.
-  - f_equal. apply H; set_solver.
-  - f_equal; [apply H | apply H0]; set_solver.
-  - f_equal; [apply H | apply H0 | apply H1]; set_solver.
+	  - f_equal. apply H; set_solver.
+	  - f_equal; [apply H | apply H0]; set_solver.
+	  - f_equal; [apply H | apply H0]; set_solver.
+	  - f_equal; [apply H | apply H0 | apply H1]; set_solver.
   - f_equal; [apply H | apply H0 | apply H1]; set_solver.
   - f_equal.
     + apply H; set_solver.
