CoreLang/theories/Sugar.v
@@ -29,6 +29,7 @@ with tm_shift (k : nat) (e : tm) : tm :=
   | tret v => tret (value_shift k v)
   | tlete e1 e2 => tlete (tm_shift k e1) (tm_shift (S k) e2)
   | tprim op v => tprim op (value_shift k v)
+  | tbinop op v1 v2 => tbinop op (value_shift k v1) (value_shift k v2)
   | tapp v1 v2 => tapp (value_shift k v1) (value_shift k v2)
   | tmatch v et ef =>
       tmatch (value_shift k v) (tm_shift k et) (tm_shift k ef)
@@ -130,6 +131,8 @@ Proof.
   - rewrite H by exact H0. reflexivity.
   - rewrite H by exact H1.
     rewrite H0 by exact H1. reflexivity.
+  - rewrite H by exact H1.
+    rewrite H0 by exact H1. reflexivity.
   - rewrite H by exact H2.
     rewrite H0 by exact H2.
     rewrite H1 by exact H2. reflexivity.
@@ -190,6 +193,8 @@ Proof.
   - rewrite H by exact H1.
     rewrite H0 by lia. reflexivity.
   - rewrite H by exact H0. reflexivity.
+  - rewrite H by exact H1.
+    rewrite H0 by exact H1. reflexivity.
   - rewrite H by exact H1.
     rewrite H0 by exact H1. reflexivity.
   - rewrite H by exact H2.
@@ -272,9 +277,10 @@ Proof.
       apply (f_equal (close_tm x 0)) in Hopen.
       rewrite !close_open_var_tm in Hopen by (rewrite ?tm_shift_fv; exact Hxfv).
       exact Hopen.
-  - rewrite H. reflexivity.
+	  - rewrite H. reflexivity.
+	  - rewrite H, H0. reflexivity.
   - rewrite H, H0. reflexivity.
-  - rewrite H, H0, H1. reflexivity.
+	  - rewrite H, H0, H1. reflexivity.
   - rewrite H, H0, H1. reflexivity.
   - f_equal.
     + rewrite H. reflexivity.
@@ -507,21 +513,28 @@ Proof.
   unfold tapp_tm.
   intros Hty.
 	  inversion Hty as
-	    [|Γ0 Tfun Tbody ef ebody L Hef Hbody| | | | | | |]; subst.
+	    [|Γ0 Tfun Tbody ef ebody L Hef Hbody| | | | | | | |]; subst.
   pose (x := fresh_for (L ∪ dom Γ ∪ fv_tm e ∪ {[y]})).
   assert (Hx : x ∉ L ∪ dom Γ ∪ fv_tm e ∪ {[y]})
     by (subst x; apply fresh_for_not_in).
   specialize (Hbody x ltac:(set_solver)).
   change (<[x:=Tfun]> Γ ⊢ₑ tapp (vfvar x) (vfvar y) ⋮ T) in Hbody.
-	  inversion Hbody as [| | |Γ1 s1 s2 v1 v2 Hfun Harg| | | | |]; subst.
-  inversion Hfun; subst.
-  rewrite lookup_insert in H1.
-  destruct (decide (x = x)); [|congruence].
-  simplify_eq.
-  exists s1. split.
-  - exact Hef.
-  - eapply basic_typing_drop_insert_fresh_value; [|exact Harg].
-    cbn [fv_value]. set_solver.
+		  inversion Hbody; subst.
+	  match goal with
+	  | Hfun : <[x:=?Tx]> Γ ⊢ᵥ vfvar x ⋮ (?s1 →ₜ T),
+	    Harg : <[x:=?Tx]> Γ ⊢ᵥ vfvar y ⋮ ?s1 |- _ =>
+	      inversion Hfun; subst;
+	      match goal with
+	      | Hlookup : <[x:=Tx]> Γ !! x = Some _ |- _ =>
+	          rewrite lookup_insert in Hlookup;
+	          destruct (decide (x = x)); [|congruence];
+	          simplify_eq;
+	          exists s1; split;
+	          [exact Hef |
+	           eapply basic_typing_drop_insert_fresh_value; [|exact Harg];
+	           cbn [fv_value]; set_solver]
+	      end
+	  end.
 Qed.
 
 Lemma basic_typing_tapp_tm_tlete_assoc Γ e1 e2 y T :
@@ -530,7 +543,7 @@ Lemma basic_typing_tapp_tm_tlete_assoc Γ e1 e2 y T :
 Proof.
   intros Hty.
 	  inversion Hty as
-	    [|Γ0 T1 T2 e1' e2' L He1 Hbody| | | | | | |]; subst.
+	    [|Γ0 T1 T2 e1' e2' L He1 Hbody| | | | | | | |]; subst.
   pose (x := fresh_for (L ∪ dom Γ ∪ fv_tm e2 ∪ {[y]})).
   assert (Hx : x ∉ L ∪ dom Γ ∪ fv_tm e2 ∪ {[y]})
     by (subst x; apply fresh_for_not_in).
@@ -568,7 +581,7 @@ Proof.
   intros Hty.
   apply basic_typing_tapp_tm_fvar_inv in Hty as [Tx [Hlet Hy]].
 	  inversion Hlet as
-	    [|Γ0 T1 T2 e1' e2' L He1 Hbody| | | | | | |]; subst.
+	    [|Γ0 T1 T2 e1' e2' L He1 Hbody| | | | | | | |]; subst.
   eapply TT_Let with (L := L ∪ dom Γ ∪ fv_tm e2 ∪ {[y]}).
   - exact He1.
   - intros z Hz.
