ProofAutomation/theories/ExtendedTypeInfer.v
@@ -1,0 +1,192 @@
+(** * Lightweight extended context-type checking for case studies *)
+
+From ProofAutomation Require Export ExtendedTyping ExtendedSubsumption BasicTypeInfer.
+From ContextTyping Require Import Typing.
+
+Open Scope core_scope.
+Open Scope case_scope.
+Open Scope cty_scope.
+Open Scope ctx_scope.
+
+Ltac extended_destruct_matches :=
+  repeat match goal with
+  | |- context[match ?x with _ => _ end] => destruct x
+  | H : context[match ?x with _ => _ end] |- _ => destruct x
+  end.
+
+Ltac extended_wf_type :=
+  match goal with
+  | |- wf_context_ty_at ?d ?D ?τ =>
+      unfold primop_precise_ty, binop_precise_ty, binop_top_ty,
+        tree_node_precise_ty, list_cons_precise_ty,
+        tree_match_eq_ty, list_match_eq_ty, precise_const, const_precise_ty,
+        precise_ty, over_ty, under_ty, primop_result_qual, binop_result_qual,
+        tree_node_result_qual, list_cons_result_qual, mk_q_eq;
+      extended_destruct_matches; case_type_wf_syntax
+  | |- basic_context_ty ?D ?τ =>
+      unfold primop_precise_ty, binop_precise_ty, binop_top_ty,
+        tree_node_precise_ty, list_cons_precise_ty,
+        tree_match_eq_ty, list_match_eq_ty, precise_const, const_precise_ty,
+        precise_ty, over_ty, under_ty, primop_result_qual, binop_result_qual,
+        tree_node_result_qual, list_cons_result_qual, mk_q_eq;
+      extended_destruct_matches; case_type_wf_syntax
+  end.
+
+Ltac extended_wf_ctx :=
+  unfold wf_ctx_under;
+  repeat
+    match goal with
+    | |- basic_ctx _ CtxEmpty => apply basic_ctx_empty
+    | |- basic_ctx _ (CtxBind _ _) =>
+        apply basic_ctx_bind; [fast_set_solver!! | extended_wf_type]
+    | |- basic_ctx _ (CtxComma _ _) =>
+        cbn [basic_ctx ctx_dom]; repeat split;
+        try extended_wf_ctx; try extended_wf_type; try fast_set_solver!!
+    | |- basic_ctx _ (CtxStar _ _) =>
+        apply basic_ctx_star; [extended_wf_ctx|extended_wf_ctx|fast_set_solver!!]
+    | |- basic_ctx _ (CtxSum _ _) =>
+        apply basic_ctx_sum; [extended_wf_ctx|extended_wf_ctx|reflexivity|reflexivity]
+    end.
+
+Ltac extended_basic_lookup :=
+  first
+    [ basic_lookup
+    | vm_compute; reflexivity ].
+
+Ltac extended_basic_value :=
+  repeat progress basic_type_surface_norm;
+  lazymatch goal with
+  | |- _ ⊢ᵥ vconst _ ⋮ _ =>
+      constructor
+  | |- _ ⊢ᵥ vfvar _ ⋮ _ =>
+      apply VT_FVar; extended_basic_lookup
+  | |- _ ⊢ᵥ avar _ ⋮ _ =>
+      change (avar _) with (vfvar _); apply VT_FVar; extended_basic_lookup
+  end.
+
+Ltac extended_basic_check :=
+  unfold ONat, UNat, OBool, UBool, OTree, UTree, OList, UList,
+    over_ty, under_ty, qual_top in *;
+  repeat rewrite erase_ctx_comma_bind_fresh by fast_set_solver!!;
+  cbn [erase_ctx erase_ty] in *;
+  repeat progress basic_type_surface_norm;
+  lazymatch goal with
+  | |- _ ⊢ₑ tprim _ _ ⋮ _ =>
+      eapply TT_Op; [cbn [prim_op_type]; reflexivity|extended_basic_value]
+  | |- _ ⊢ₑ tbinop _ _ _ ⋮ _ =>
+      eapply TT_BinOp; [basic_solve_binop_type|extended_basic_value|extended_basic_value]
+  | |- _ ⊢ₑ tret _ ⋮ _ =>
+      apply TT_Ret; extended_basic_value
+  | |- _ ⊢ₑ tnode _ _ _ ⋮ _ =>
+      eapply TT_TreeNode; extended_basic_value
+  | |- _ ⊢ₑ tcons _ _ ⋮ _ =>
+      eapply TT_ListCons; extended_basic_value
+  | |- _ ⊢ₑ _ ⋮ _ =>
+      basic_check
+  end.
+
+Ltac extended_wf :=
+  unfold context_typing_wf;
+  repeat split;
+  try solve
+    [ extended_wf_ctx
+    | extended_wf_type
+    | fast_set_solver!!
+    | extended_basic_check
+    | unfold ONat, UNat, OBool, UBool, OTree, UTree, OList, UList,
+        over_ty, under_ty, qual_top in *;
+      repeat rewrite erase_ctx_comma_bind_fresh by fast_set_solver!!;
+      cbn [erase_ctx erase_ty] in *; basic_type ].
+
+Ltac extended_case_surface_norm :=
+  unfold Ret, avar, vbool, vnat, leaf_value, nil_value, vlist in *;
+  cbn [Ret prim_op_type bin_op_type base_ty_of_const] in *;
+  lazymatch goal with
+  | |- context[tret (vfvar ?x)] =>
+      change (tret (vfvar x)) with (tret (avar x))
+  | _ => idtac
+  end.
+
+Ltac extended_check_fuel fuel :=
+  lazymatch fuel with
+  | O => fail "extended_check_fuel: fuel exhausted"
+  | S ?fuel' =>
+  extended_case_surface_norm;
+  lazymatch goal with
+  | |- ?Σ ; Emp ⊢ₓ ret (vconst ?c) ⋮ const_precise_ty ?c =>
+      eapply EXT_Const; extended_wf
+  | |- ?Σ ; Emp ⊢ₓ tret (vconst ?c) ⋮ const_precise_ty ?c =>
+      change (tret (vconst c)) with (ret (vconst c));
+      eapply EXT_Const; extended_wf
+  | |- ?Σ ; Emp ⊢ₓ ret ?v ⋮ const_precise_ty ?c =>
+      change v with (vconst c);
+      eapply EXT_Const; extended_wf
+  | Hsub : sub_type_under ?Σ ?Γ ?τ1 ?τ2
+      |- ?Σ ; ?Γ ⊢ₓ ?e ⋮ ?τ2 =>
+      eapply EXT_Sub;
+      [extended_wf|extended_check_fuel fuel'|exact Hsub]
+  | |- ?Σ ; ?x ∷ ?τ ⊢ₓ ret (avar ?x) ⋮ ?τ =>
+      eapply EXT_Var; extended_wf
+  | |- ?Σ ; ?Γ ⊢ₓ ?v1 ⟨ ?op ⟩ ?v2 ⋮ binop_precise_ty ?op ?v1 ?v2 =>
+      eapply EXT_BinOp; extended_wf
+  | |- ?Σ ; ?Γ ⊢ₓ ?v1 ⟨ ?op ⟩ ?v2 ⋮ binop_top_ty ?op =>
+      eapply EXT_BinOpTop; extended_wf
+  | |- ?Σ ; ?Γ ⊢ₓ ?op ·₁ ?v ⋮ primop_precise_ty ?op ?v =>
+      eapply EXT_AppOpValue; extended_wf
+  | |- ?Σ ; ?Γ ⊢ₓ ?f @ ?x ⋮ ?τ =>
+      eapply EXT_AppFun with (τx := ONat);
+      [extended_wf|fast_set_solver!!|extended_check_fuel fuel'|extended_check_fuel fuel']
+  | |- ?Σ ; ?Γ ⊢ₓ ret (vlam ?Tx (close_tm ?x 0 ?e)) ⋮ (?τx → ?τ) =>
+      change (ret (vlam Tx (close_tm x 0 e)))
+        with (ret (lam_named x Tx e));
+      eapply EXT_LamNamedErased;
+      [unfold ONat, UNat, OBool, UBool, OTree, UTree, OList, UList,
+         base_ty_as_ty, over_ty, under_ty, qual_top;
+       cbn [erase_ty]; reflexivity|extended_wf|extended_check_fuel fuel']
+  | |- ?Σ ; ?Γ ⊢ₓ ret (lam_named ?x ?Tx ?e) ⋮ (?τx → ?τ) =>
+      eapply EXT_LamNamedErased;
+      [unfold ONat, UNat, OBool, UBool, OTree, UTree, OList, UList,
+         base_ty_as_ty, over_ty, under_ty, qual_top;
+       cbn [erase_ty]; reflexivity|extended_wf|extended_check_fuel fuel']
+  | |- ?Σ ; ?Γ ⊢ₓ tlete ?e1 (close_tm ?x 0 ?e2) ⋮ ?τ =>
+      change (tlete e1 (close_tm x 0 e2)) with (let_named x e1 e2);
+      eapply EXT_LetNamed; [extended_wf|extended_check_fuel fuel'|extended_check_fuel fuel']
+  | |- ?Σ ; ?Γ ⊢ₓ let ?x := ?e1 in ?e2 ⋮ ?τ =>
+      eapply EXT_LetNamed; [extended_wf|extended_check_fuel fuel'|extended_check_fuel fuel']
+  | |- ?Σ ; ?Γ ⊢ₓ [| ?root, ?left, ?right |] ⋮
+        tree_node_precise_ty ?root ?left ?right =>
+      eapply EXT_TreeNode;
+      [extended_wf|extended_check_fuel fuel'|extended_check_fuel fuel'|extended_check_fuel fuel']
+  | |- ?Σ ; ?Γ ⊢ₓ ?hd ::ᵗ ?tl ⋮ list_cons_precise_ty ?hd ?tl =>
+      eapply EXT_ListCons; [extended_wf|extended_check_fuel fuel'|extended_check_fuel fuel']
+  | |- ?Σ ; ?Γ ⊢ₓ ret ?v ⋮ ?τ =>
+      eapply typing_to_extended_typing;
+      eauto using has_context_type
+  | |- ?Σ ; ?Γ ⊢ₓ ?e ⋮ ?τ =>
+      eapply typing_to_extended_typing;
+      eauto using has_context_type
+  end
+  end.
+
+Ltac extended_check := extended_check_fuel 16.
+
+Section Regression.
+
+  Lemma extended_check_const_nat :
+    ∅; Emp ⊢ₓ ret (vnat 1) ⋮ const_precise_ty (cnat 1).
+  Proof.
+    eapply EXT_Const.
+    unfold context_typing_wf.
+    repeat split; try extended_wf_type; try fast_set_solver!!.
+  Qed.
+
+  Lemma extended_check_binop_nat :
+    ∅; (1%positive ∷ ONat) ,, (2%positive ∷ ONat) ⊢ₓ
+      avar 1%positive ⟨ + ⟩ avar 2%positive ⋮
+      binop_precise_ty bop_plus (avar 1%positive) (avar 2%positive).
+  Proof.
+    eapply EXT_BinOp.
+    extended_wf.
+  Qed.
+
+End Regression.
